src/util/Tactics.v
@@ -1,0 +1,19 @@
+Require Import Coq.omega.Omega.
+
+(* Like "pose proof" but only if we don't yet have this hypothesis *)
+Tactic Notation "unique" "pose" "proof" constr(defn) :=
+  let T := type of defn in
+  match goal with
+  | [ H : T |- _ ] => fail 1
+  | _ => pose proof defn
+  end.
+
+(* Like "omega" but also knows about min and max *)
+Ltac momega :=
+  repeat match goal with
+         | _: context[min ?a ?b] |- _ => unique pose proof (Min.min_spec a b)
+         |  |- context[min ?a ?b]     => unique pose proof (Min.min_spec a b)
+         | _: context[max ?a ?b] |- _ => unique pose proof (Max.max_spec a b)
+         |  |- context[max ?a ?b]     => unique pose proof (Max.max_spec a b)
+  end;
+  omega.
